Weidenbach_Book/IsaSAT_Conflict_Analysis.thy
@@ -40,7 +40,6 @@ lemma get_conflict_wll_is_Nil_code_get_conflict_wl_is_Nil[sepref_fr_rules]:
 definition (in -) get_count_max_lvls_code where
   \<open>get_count_max_lvls_code = (\<lambda>(_, _, _, _, _, _, _, _, clvls, _). clvls)\<close>
 
-
 lemma get_count_max_lvls_heur_hnr[sepref_fr_rules]:
   \<open>(return o get_count_max_lvls_code, RETURN o get_count_max_lvls_heur) \<in>
      twl_st_heur_assn\<^sup>k \<rightarrow>\<^sub>a uint32_nat_assn\<close>
@@ -70,8 +69,7 @@ lemmas maximum_level_removed_eq_count_dec_code_hnr[sepref_fr_rules] =
 sepref_thm is_decided_hd_trail_wl_code
   is \<open>RETURN o is_decided_hd_trail_wl_heur\<close>
   :: \<open>[\<lambda>S. get_trail_wl_heur S \<noteq> []]\<^sub>a twl_st_heur_assn\<^sup>k \<rightarrow> bool_assn\<close>
-  unfolding is_decided_hd_trail_wl_heur_def twl_st_heur_assn_def
-    supply get_trail_wl_heur_def[simp]
+  unfolding is_decided_hd_trail_wl_heur_alt_def twl_st_heur_assn_def
   by sepref
 
 
@@ -111,18 +109,15 @@ setup \<open>map_theory_claset (fn ctxt => ctxt addSbefore ("split_all_tac", spl
 context isasat_input_bounded_nempty
 begin
 
-
 sepref_thm tl_state_wl_heur_code
   is \<open>RETURN o tl_state_wl_heur\<close>
-  :: \<open>[\<lambda>(M, N, U, D, WS, Q, ((A, m, fst_As, lst_As, next_search), _), \<phi>, _). M \<noteq> [] \<and>
-         atm_of (lit_of (hd M)) < length \<phi> \<and>
-         atm_of (lit_of (hd M)) < length A \<and> (next_search \<noteq> None \<longrightarrow>  the next_search < length A)]\<^sub>a
+  :: \<open>[tl_state_wl_heur_pre]\<^sub>a
       twl_st_heur_assn\<^sup>d \<rightarrow> twl_st_heur_assn\<close>
   supply [[goals_limit=1]] option.splits[split] if_splits[split]
   option.splits[split]
   supply [[goals_limit=1]] option.splits[split] literals_are_\<L>\<^sub>i\<^sub>n_hd_trail_in_D\<^sub>0[intro]
   unfolding tl_state_wl_heur_alt_def[abs_def] twl_st_heur_assn_def get_trail_wl_heur_def[simp]
-    vmtf_unset_def bind_ref_tag_def[simp]
+    vmtf_unset_def bind_ref_tag_def[simp] tl_state_wl_heur_pre_def
     short_circuit_conv
   by sepref
 
@@ -212,28 +207,12 @@ lemma lookup_clause_assn_op_nset_is_emty[sepref_fr_rules]:
 
 sepref_thm update_confl_tl_wl_code
   is \<open>uncurry2 update_confl_tl_wl_heur\<close>
-  :: \<open>[\<lambda>((i, L), (M, N, U, D, W, Q, ((A, m, fst_As, lst_As, next_search), _), \<phi>, clvls, cach)).
-      (i > 0 \<longrightarrow> distinct (N ! i)) \<and>
-      (i > 0 \<longrightarrow> literals_are_in_\<L>\<^sub>i\<^sub>n (mset (N! i))) \<and>
-      (i > 0 \<longrightarrow> \<not> tautology (mset (N ! i))) \<and>
-      i < length N \<and> \<not> tautology (the D) \<and>
-      literals_are_in_\<L>\<^sub>i\<^sub>n (the D) \<and> D \<noteq> None \<and>
-      M \<noteq> [] \<and>
-      L \<in> snd ` D\<^sub>0 \<and> -L \<in># the D \<and> L \<notin># the D \<and>
-      (i > 0 \<longrightarrow> (L \<in> set (N ! i) \<and> -L \<notin> set (N ! i))) \<and>
-      (i > 0 \<longrightarrow> (\<forall>L \<in> set (tl (N ! i)). - L \<notin># the D)) \<and>
-      (i > 0 \<longrightarrow> card_max_lvl M (mset (tl (N ! i)) \<union># the D) \<ge> 1) \<and>
-      atm_of (lit_of (hd M)) < length \<phi> \<and>
-      atm_of (lit_of (hd M)) < length A \<and> (next_search \<noteq> None \<longrightarrow>  the next_search < length A) \<and>
-      L = lit_of (hd M) \<and>
-      clvls = card_max_lvl M (the D) \<and>
-      literals_are_in_\<L>\<^sub>i\<^sub>n_trail M \<and>
-      no_dup M
-         ]\<^sub>a
+  :: \<open>[update_confl_tl_wl_heur_pre]\<^sub>a
   nat_assn\<^sup>k *\<^sub>a unat_lit_assn\<^sup>k *\<^sub>a twl_st_heur_assn\<^sup>d \<rightarrow> bool_assn *a twl_st_heur_assn\<close>
   supply image_image[simp] uminus_\<A>\<^sub>i\<^sub>n_iff[iff] in_diffD[dest] option.splits[split]
   supply [[goals_limit=1]]
   unfolding update_confl_tl_wl_heur_def twl_st_heur_assn_def save_phase_def
+    update_confl_tl_wl_heur_pre_def
   supply merge_conflict_m_def[simp]
   by sepref (* slow *)
 
@@ -245,187 +224,6 @@ prepare_code_thms (in -) update_confl_tl_wl_code_def
 
 lemmas update_confl_tl_wl_code_refine[sepref_fr_rules] =
    update_confl_tl_wl_code.refine[of \<A>\<^sub>i\<^sub>n, OF isasat_input_bounded_nempty_axioms]
-(* 
-lemma update_confl_tl_wl_code_update_confl_tl_wl[sepref_fr_rules]:
-  \<open>(uncurry2 update_confl_tl_wl_code, uncurry2 (RETURN ooo update_confl_tl_wl))
-    \<in> [\<lambda>((C, L), S). twl_struct_invs (twl_st_of_wl None S) \<and>
-        twl_stgy_invs (twl_st_of_wl None S) \<and>
-        get_conflict_wl S \<noteq> None \<and>
-        get_trail_wl S \<noteq> [] \<and>
-        - L \<in># the (get_conflict_wl S) \<and>
-        (L, C) = lit_and_ann_of_propagated_st S \<and>
-        literals_are_\<L>\<^sub>i\<^sub>n S \<and>
-        is_proped (hd (get_trail_wl S)) \<and>
-        twl_list_invs (st_l_of_wl None S)]\<^sub>a
-       nat_assn\<^sup>k *\<^sub>a unat_lit_assn\<^sup>k *\<^sub>a twl_st_assn\<^sup>d \<rightarrow> bool_assn *a twl_st_assn\<close>
-  (is \<open>?c \<in> [?pre]\<^sub>a ?im \<rightarrow> ?f\<close>)
-proof -
-  have H: \<open>?c \<in>  [comp_PRE (nat_rel \<times>\<^sub>f nat_lit_lit_rel \<times>\<^sub>f twl_st_heur)
-     (\<lambda>((C, L), S).
-         twl_struct_invs (twl_st_of_wl None S) \<and>
-         twl_stgy_invs (twl_st_of_wl None S) \<and>
-         twl_list_invs (st_l_of_wl None S) \<and>
-         C < length (get_clauses_wl S) \<and>
-         get_conflict_wl S \<noteq> None \<and>
-         get_trail_wl S \<noteq> [] \<and>
-         - L \<in># the (get_conflict_wl S) \<and>
-         (L, C) =
-         lit_and_ann_of_propagated (hd (get_trail_wl S)) \<and>
-         L \<in> snd ` D\<^sub>0 \<and> is_proped (hd (get_trail_wl S)))
-     (\<lambda>_ ((i, L), M, N, U, D, W, Q, ((A, m, fst_As, lst_As,
-         next_search), _), \<phi>, clvls, cach).
-         (0 < i \<longrightarrow> distinct (N ! i)) \<and>
-         (0 < i \<longrightarrow> literals_are_in_\<L>\<^sub>i\<^sub>n (mset (N ! i))) \<and>
-         (0 < i \<longrightarrow> \<not> tautology (mset (N ! i))) \<and>
-         i < length N \<and>
-         \<not> tautology (the D) \<and>
-         literals_are_in_\<L>\<^sub>i\<^sub>n (the D) \<and>
-         D \<noteq> None \<and>
-         M \<noteq> [] \<and>
-         L \<in> snd ` D\<^sub>0 \<and>
-         - L \<in># the D \<and>
-         L \<notin># the D \<and>
-         (0 < i \<longrightarrow> L \<in> set (N ! i) \<and> - L \<notin> set (N ! i)) \<and>
-         (0 < i \<longrightarrow> (\<forall>L\<in>set (tl (N ! i)). - L \<notin># the D)) \<and>
-         (0 < i \<longrightarrow>
-          1 \<le> card_max_lvl M (mset (tl (N ! i)) \<union># the D)) \<and>
-         atm_of (lit_of (hd M)) < length \<phi> \<and>
-         atm_of (lit_of (hd M)) < length A \<and>
-         (next_search \<noteq> None \<longrightarrow> the next_search < length A) \<and>
-         L = lit_of (hd M) \<and>
-         clvls = card_max_lvl M (the D) \<and>
-         literals_are_in_\<L>\<^sub>i\<^sub>n_trail M \<and> no_dup M)
-     (\<lambda>_. True)]\<^sub>a hrp_comp
-                     (nat_assn\<^sup>k *\<^sub>a unat_lit_assn\<^sup>k *\<^sub>a
-                      twl_st_heur_assn\<^sup>d)
-                     (nat_rel \<times>\<^sub>f nat_lit_lit_rel \<times>\<^sub>f
-                      twl_st_heur) \<rightarrow> hr_comp
-      (bool_assn *a twl_st_heur_assn) (bool_rel \<times>\<^sub>f twl_st_heur)\<close>
-      (is \<open>_ \<in> [?pre']\<^sub>a ?im' \<rightarrow> ?f'\<close>)
-    using hfref_compI_PRE_aux[OF update_confl_tl_wl_code_refine
-       update_confl_tl_wl_heur_update_confl_tl_wl]
-    .
-  have pre: \<open>?pre' x\<close> (is \<open>comp_PRE ?rel ?\<Phi> ?\<Psi> _ x\<close>) if pre: \<open>?pre x\<close> for x
-  unfolding comp_PRE_def
-  proof (intro allI impI conjI)
-    obtain C L S where
-      [simp]: \<open>x = ((C,L), S)\<close>
-      by (cases x) auto
-    obtain M N U D W Q NE UE where
-      [simp]: \<open>S = (M, N, U, D, NE, UE, W, Q)\<close>
-      by (cases S) auto
-    have LC: \<open>(L, C) = lit_and_ann_of_propagated (hd (get_trail_wl S))\<close> and
-      lits_\<A>\<^sub>i\<^sub>n: \<open>literals_are_\<L>\<^sub>i\<^sub>n S\<close> and
-      struct_invs: \<open>twl_struct_invs (twl_st_of None (st_l_of_wl None S))\<close> and
-      list_invs: \<open>twl_list_invs (st_l_of_wl None S)\<close> and
-      trail_nempty: \<open>get_trail_wl S \<noteq> []\<close> and
-      add_invs: \<open>twl_list_invs (st_l_of_wl None S)\<close> and
-      proped: \<open>is_proped (hd (get_trail_wl S))\<close> and
-      confl: \<open>get_conflict_wl S \<noteq> None\<close> and
-      L_confl: \<open>-L \<in># the(get_conflict_wl S)\<close>
-      using that by (auto simp: lit_and_ann_of_propagated_st_def)
-    have lits_D: \<open>literals_are_in_\<L>\<^sub>i\<^sub>n (the (get_conflict_wl S))\<close>
-      by (rule literals_are_\<L>\<^sub>i\<^sub>n_conflict_literals_are_in_\<L>\<^sub>i\<^sub>n[of _ None])
-       (use lits_\<A>\<^sub>i\<^sub>n confl struct_invs in auto)
-    have C_le: \<open>C < length (get_clauses_wl S)\<close>
-      using trail_nempty LC proped add_invs trail_nempty unfolding twl_list_invs_def
-      by (cases M; cases \<open>hd M\<close>) auto
-    moreover have L_D\<^sub>0: \<open>L \<in> snd ` D\<^sub>0\<close>
-      using L_confl confl lits_D
-      by (cases \<open>get_conflict_wl S\<close>)
-        (auto simp: image_image literals_are_in_\<L>\<^sub>i\<^sub>n_add_mset uminus_\<A>\<^sub>i\<^sub>n_iff
-            dest: multi_member_split)
-    ultimately show \<open>?\<Phi> x\<close>
-      using that by (auto simp: lit_and_ann_of_propagated_st_def)
-    have
-      trail: \<open>literals_are_in_\<L>\<^sub>i\<^sub>n_trail( get_trail_wl S)\<close>
-      using literals_are_\<L>\<^sub>i\<^sub>n_literals_are_in_\<L>\<^sub>i\<^sub>n_trail[OF lits_\<A>\<^sub>i\<^sub>n, of None ] struct_invs
-      by auto
-
-    fix x'
-    assume x'x: \<open>(x', x) \<in> nat_rel \<times>\<^sub>f Id \<times>\<^sub>f twl_st_heur\<close>
-    then obtain S' where
-      [simp]: \<open>x' = ((C, L), S')\<close>
-      by (cases x') auto
-    obtain Q' A m fst_As lst_As next_search oth \<phi> clvls cach where
-      [simp]: \<open>S' = (M, N, U, D, W, Q', ((A, m, fst_As, lst_As, next_search), oth), \<phi>, clvls, cach)\<close> and
-      n_d: \<open>no_dup (get_trail_wl S)\<close>
-      using x'x by (cases S') (auto simp: twl_st_heur_def)
-    have in_atms_le: \<open>\<forall>L\<in>atms_of \<L>\<^sub>a\<^sub>l\<^sub>l. L < length A\<close> and \<phi>: \<open>phase_saving \<phi>\<close> and
-      vmtf: \<open>\<exists>xs' ys'. vmtf_ns (ys' @ xs') m A \<and> fst_As = hd (ys' @ xs') \<and>
-           lst_As = last (ys' @ xs') \<and> next_search = option_hd xs'\<close> and
-      clvls: \<open>clvls \<in> counts_maximum_level M D\<close>
-      using x'x unfolding twl_st_heur_def vmtf_def by auto
-    then have atm_L_le_A: \<open>atm_of L < length A\<close>
-      using L_D\<^sub>0 by (auto simp: image_image in_\<L>\<^sub>a\<^sub>l\<^sub>l_atm_of_in_atms_of_iff)
-    have atm_L_le_\<phi>: \<open>atm_of L < length \<phi>\<close>
-      using L_D\<^sub>0 \<phi> unfolding phase_saving_def by (auto simp: image_image in_\<L>\<^sub>a\<^sub>l\<^sub>l_atm_of_in_atms_of_iff)
-    obtain xs' ys' where
-      \<open>vmtf_ns (ys' @ xs') m A\<close> and \<open>fst_As = hd (ys' @ xs')\<close> and \<open>next_search = option_hd xs'\<close> and
-      \<open>lst_As = last (ys' @ xs')\<close>
-      using vmtf by blast
-    then have next_search: \<open>the next_search < length A\<close> if \<open>next_search \<noteq> None\<close>
-      apply - by (rule vmtf_ns_le_length[of \<open>ys' @ xs'\<close> m A]) (use that in auto)
-    have \<open>cdcl\<^sub>W_restart_mset.cdcl\<^sub>W_all_struct_inv (state\<^sub>W_of (twl_st_of None (st_l_of_wl None S)))\<close>
-      using struct_invs unfolding twl_struct_invs_def by fast
-    then have \<open>cdcl\<^sub>W_restart_mset.distinct_cdcl\<^sub>W_state (state\<^sub>W_of (twl_st_of None (st_l_of_wl None S)))\<close>
-      unfolding cdcl\<^sub>W_restart_mset.cdcl\<^sub>W_all_struct_inv_def by fast+
-    then have \<open>distinct_mset_set (mset ` set (tl N))\<close>
-      apply (subst append_take_drop_id[of U, symmetric])
-      unfolding set_append image_Un
-      by (auto simp: cdcl\<^sub>W_restart_mset.distinct_cdcl\<^sub>W_state_def mset_take_mset_drop_mset drop_Suc)
-    then have dist_NC: \<open>distinct (N ! C)\<close> if \<open>C > 0\<close>
-      using that C_le nth_in_set_tl[of C N] by (auto simp: distinct_mset_set_def)
-
-    have lits_NC: \<open>literals_are_in_\<L>\<^sub>i\<^sub>n (mset (N ! C))\<close> if \<open>C > 0\<close>
-      by (rule literals_are_in_\<L>\<^sub>i\<^sub>n_nth) (use C_le that lits_\<A>\<^sub>i\<^sub>n in auto)
-    have L_hd_M: \<open>L = lit_of (hd M)\<close>
-      by (cases M; cases \<open>hd M\<close>) (use trail_nempty LC proped in auto)
-
-    have tauto_confl: \<open>\<not> tautology (the (get_conflict_wl S))\<close>
-      using resolve_cls_wl'_not_tauto_confl[of S C L] struct_invs confl L_confl C_le trail_nempty
-      proped LC list_invs by auto
-    have L_notin_D: \<open>L \<notin># the D\<close>
-      using resolve_cls_wl'_not_tauto_confl[of S C L] struct_invs confl L_confl C_le trail_nempty
-      proped LC list_invs by auto
-    have tauto: \<open>\<not>tautology (mset (N ! C))\<close> if \<open>C > 0\<close>
-      using resolve_cls_wl'_not_tauto_cls[of S C L] struct_invs confl L_confl C_le trail_nempty
-      proped LC that list_invs
-      by auto
-    have L_NC: \<open>L \<in> set (N ! C)\<close> if \<open>C > 0\<close>
-      using resolve_cls_wl'_L_in_cls[of S C L] struct_invs confl L_confl C_le trail_nempty
-      proped LC that list_invs by auto
-    have L_NC': \<open>-L \<notin> set (N ! C)\<close> if \<open>C > 0\<close>
-      using tauto that L_NC apply (auto simp: tautology_decomp)
-      by (metis (full_types) nat_of_lit.cases uminus_Pos uminus_of_uminus_id)
-    have [simp]: \<open>Suc 0 \<le> card_max_lvl M (mset (tl (N ! C)) \<union># the D)\<close>
-      if \<open>C > 0\<close>
-      using resolve_cls_wl'_card_max_lvl[of S C L] LC confl C_le L_D\<^sub>0 clvls that pre
-      by (auto simp: counts_maximum_level_def)
-    have \<open>C > 0 \<Longrightarrow> La \<in> set (tl (N ! C)) \<Longrightarrow> - La \<in># the D \<Longrightarrow> False\<close> for La
-      using resolve_helper_seperated[of S C L] struct_invs confl L_confl C_le trail_nempty
-      proped LC that list_invs
-      by auto
-    then show \<open>?\<Psi> x x'\<close>
-      using confl L_confl dist_NC lits_NC C_le trail_nempty L_D\<^sub>0 tauto lits_D L_notin_D L_NC
-      atm_L_le_A atm_L_le_\<phi> next_search clvls tauto_confl
-      trail n_d
-      by (auto simp: L_hd_M[symmetric] counts_maximum_level_def)
-  qed
-  have im: \<open>?im' = ?im\<close>
-    unfolding prod_hrp_comp hrp_comp_dest hrp_comp_keep twl_st_assn_def
-    by (auto simp: hrp_comp_def hr_comp_def)
-  have f: \<open>?f' = ?f\<close>
-    unfolding prod_hrp_comp hrp_comp_dest hrp_comp_keep twl_st_assn_def hr_comp_prod_conv
-      lookup_clause_assn_def
-    by (auto simp: hrp_comp_def hr_comp_def)
-  show ?thesis
-    apply (rule hfref_weaken_pre[OF ])
-     defer
-    using H unfolding im f PR_CONST_def apply assumption
-    using pre ..
-qed
- *)
 
 end
 
@@ -435,10 +233,16 @@ setup \<open>map_theory_claset (fn ctxt => ctxt delSWrapper ("split_all_tac"))\<
 context isasat_input_bounded_nempty
 begin
 
+lemma skip_and_resolve_loop_wl_D_heur_inv_nempty:
+  \<open>skip_and_resolve_loop_wl_D_heur_inv S\<^sub>0 (brk, S) \<Longrightarrow> \<not>brk \<Longrightarrow> get_trail_wl_heur S \<noteq> []\<close>
+  unfolding skip_and_resolve_loop_wl_D_heur_inv_def skip_and_resolve_loop_wl_D_inv_def
+    skip_and_resolve_loop_inv_def
+   by (auto simp: twl_st_heur_def)
+
 sepref_register skip_and_resolve_loop_wl_D is_in_conflict_st
 sepref_thm skip_and_resolve_loop_wl_D
-  is \<open>PR_CONST skip_and_resolve_loop_wl_D\<close>
-  :: \<open>twl_st_assn\<^sup>d \<rightarrow>\<^sub>a twl_st_assn\<close>
+  is \<open>PR_CONST skip_and_resolve_loop_wl_D_heur\<close>
+  :: \<open>twl_st_heur_assn\<^sup>d \<rightarrow>\<^sub>a twl_st_heur_assn\<close>
   supply [[goals_limit=1]] get_trail_twl_st_of_wl_get_trail_wl_empty_iff[simp]
     is_decided_hd_trail_wl_def[simp]
     is_decided_no_proped_iff[simp] skip_and_resolve_hd_in_D\<^sub>0[intro]
@@ -448,26 +252,11 @@ sepref_thm skip_and_resolve_loop_wl_D
     annotated_lit.disc_eq_case(2)[simp]
     skip_and_resolde_hd_D\<^sub>0[simp]
     not_None_eq[simp del] maximum_level_removed_eq_count_dec_def[simp]
+    skip_and_resolve_loop_wl_D_heur_inv_nempty[simp]
+    is_decided_hd_trail_wl_heur_def[simp]
   apply (subst PR_CONST_def)
-  unfolding skip_and_resolve_loop_wl_D_def
+  unfolding skip_and_resolve_loop_wl_D_heur_def
   apply (rewrite at \<open>\<not>_ \<and> \<not> _\<close> short_circuit_conv)
-  apply (rewrite at \<open>let _ = the _ in _\<close> Let_def)
-  unfolding
-    maximum_level_removed_eq_count_dec_def[unfolded get_maximum_level_remove_def, symmetric]
-  unfolding
-    literals_to_update_wl_literals_to_update_wl_empty
-    get_conflict_wl.simps get_trail_wl.simps
-    maximum_level_removed_eq_count_dec_def[symmetric]
-    is_decided_hd_trail_wl_def[symmetric]
-    skip_and_resolve_loop_inv_def
-    Multiset.is_empty_def[symmetric]
-    get_maximum_level_remove_def[symmetric]
-    is_in_conflict_st_def[symmetric]
-    lit_and_ann_of_propagated_st_def[symmetric]
-    get_max_lvl_st_def[symmetric]
-    count_decided_st_alt_def[symmetric]
-    get_conflict_wl_get_conflict_wl_is_Nil
-    is_in_conflict_def[symmetric]
   by sepref (* slow *)
 
 concrete_definition (in -) skip_and_resolve_loop_wl_D_code
